etl

coq_effect/etl_ast.v
@@ -13,13 +13,17 @@ Open Scope sort_scope.
 Inductive term : Type :=
 | Var (x : var)
 | Ty
-| Forall0 (A : term) (B : {bind term}) (* ∀{x : A}.B *)
-| Forall1 (A : term) (B : {bind term}) (* ∀(x : A).B *)
-| Arrow   (A : term) (B : term)        (* A → B      *)
-| Lam0 (A : term) (m : {bind term})    (* Λ{x : A}.m *)
-| Lam1 (A : term) (m : {bind term})    (* Λ(x : A).m *)
-| Fun (A : term) (m : {bind term})     (* λ(x : A).m *)
-| App (m n : term)                     (* m n *).
+| Forall (A : term) (B : {bind term}) (* ∀(x : A).B *)
+| Arrow  (A : term) (B : term)        (* A → B      *)
+| Lam  (A : term) (m : {bind term})   (* Λ(x : A).m *)
+| Fun  (A : term) (m : {bind term})   (* λ(x : A).m *)
+| Inst (m n : term)                   (* m<n> *)
+| Call (m n : term)                   (* m(n) *)
+| UnitT
+| Unit
+| NatT
+| Nat (n : nat)
+| Rand (m : term).
 
 #[global] Instance Ids_term : Ids term. derive. Defined.
 #[global] Instance Rename_term : Rename term. derive. Defined.
