coq_effect/sta_type.v
@@ -6,247 +6,72 @@ Set Implicit Arguments.
 Unset Strict Implicit.
 Unset Printing Implicit Defensive.
 
-Inductive sta0_type : sta_ctx -> term -> term -> Prop :=
-| sta0_axiom Γ s l :
-  sta0_wf Γ ->
-  sta0_type Γ (Sort s l) (Sort U l.+1)
-| sta0_var Γ x A :
-  sta0_wf Γ ->
-  sta_has Γ x A ->
-  sta0_type Γ (Var x) A
-| sta0_pi0 Γ A B s r t l1 l2 :
-  sta0_type Γ A (Sort r l1) ->
-  sta0_type (A :: Γ) B (Sort t l2) ->
-  sta0_type Γ (Pi0 A B s) (Sort s (maxn l1 l2))
-| sta0_pi1 Γ A B s r t l1 l2 :
-  sta0_type Γ A (Sort r l1) ->
-  sta0_type (A :: Γ) B (Sort t l2) ->
-  sta0_type Γ (Pi1 A B s) (Sort s (maxn l1 l2))
-| sta0_lam0 Γ A B m s r l :
-  sta0_type Γ A (Sort r l) ->
-  sta0_type (A :: Γ) m B ->
-  sta0_type Γ (Lam0 A m s) (Pi0 A B s)
-| sta0_lam1 Γ A B m s r l :
-  sta0_type Γ A (Sort r l) ->
-  sta0_type (A :: Γ) m B ->
-  sta0_type Γ (Lam1 A m s) (Pi1 A B s)
-| sta0_app0 Γ A B m n s :
-  sta0_type Γ m (Pi0 A B s) ->
-  sta0_type Γ n A ->
-  sta0_type Γ (App m n) B.[n/]
-| sta0_app1 Γ A B m n s :
-  sta0_type Γ m (Pi1 A B s) ->
-  sta0_type Γ n A ->
-  sta0_type Γ (App m n) B.[n/]
-| sta0_sig0 Γ A B s r t l1 l2 :
-  s ⊑ t ->
-  sta0_type Γ A (Sort s l1) ->
-  sta0_type (A :: Γ) B (Sort r l2) ->
-  sta0_type Γ (Sig0 A B t) (Sort t (maxn l1 l2))
-| sta0_sig1 Γ A B s r t l1 l2 :
-  s ⊑ t ->
-  r ⊑ t ->
-  sta0_type Γ A (Sort s l1) ->
-  sta0_type (A :: Γ) B (Sort r l2) ->
-  sta0_type Γ (Sig1 A B t) (Sort t (maxn l1 l2))
-| sta0_pair0 Γ A B m n t l :
-  sta0_type Γ (Sig0 A B t) (Sort t l) ->
-  sta0_type Γ m A ->
-  sta0_type Γ n B.[m/] ->
-  sta0_type Γ (Pair0 m n t) (Sig0 A B t)
-| sta0_pair1 Γ A B m n t l :
-  sta0_type Γ (Sig1 A B t) (Sort t l) ->
-  sta0_type Γ m A ->
-  sta0_type Γ n B.[m/] ->
-  sta0_type Γ (Pair1 m n t) (Sig1 A B t)
-| sta0_letin0 Γ A B C m n s t l :
-  sta0_type (Sig0 A B t :: Γ) C (Sort s l) ->
-  sta0_type Γ m (Sig0 A B t) ->
-  sta0_type (B :: A :: Γ) n C.[Pair0 (Var 1) (Var 0) t .: ren (+2)] ->
-  sta0_type Γ (LetIn C m n) C.[m/]
-| sta0_letin1 Γ A B C m n s t l :
-  sta0_type (Sig1 A B t :: Γ) C (Sort s l) ->
-  sta0_type Γ m (Sig1 A B t) ->
-  sta0_type (B :: A :: Γ) n C.[Pair1 (Var 1) (Var 0) t .: ren (+2)] ->
-  sta0_type Γ (LetIn C m n) C.[m/]
-| sta0_with Γ A B s r t l1 l2 :
-  sta0_type Γ A (Sort s l1) ->
-  sta0_type Γ B (Sort r l2) ->
-  sta0_type Γ (With A B t) (Sort t (maxn l1 l2))
-| sta0_apair Γ A B m n t :
-  sta0_type Γ m A ->
-  sta0_type Γ n B ->
-  sta0_type Γ (APair m n t) (With A B t)
-| sta0_fst Γ A B m t :
-  sta0_type Γ m (With A B t) ->
-  sta0_type Γ (Fst m) A
-| sta0_snd Γ A B m t :
-  sta0_type Γ m (With A B t) ->
-  sta0_type Γ (Snd m) B
-| sta0_id Γ A m n s l :
-  sta0_type Γ A (Sort s l) ->
-  sta0_type Γ m A ->
-  sta0_type Γ n A ->
-  sta0_type Γ (Id A m n) (Sort U l)
-| sta0_refl Γ A m :
-  sta0_type Γ m A ->
-  sta0_type Γ (Refl m) (Id A m m)
-| sta0_rw Γ A B H P m n s l :
-  sta0_type (Id A.[ren (+1)] m.[ren (+1)] (Var 0) :: A :: Γ) B (Sort s l) ->
-  sta0_type Γ H B.[Refl m,m/] ->
-  sta0_type Γ P (Id A m n) ->
-  sta0_type Γ (Rw B H P) B.[P,n/]
-| sta0_conv Γ A B m s l :
-  A === B ->
-  sta0_type Γ m A ->
-  sta0_type Γ B (Sort s l) ->
-  sta0_type Γ m B
-
-with sta0_wf : sta_ctx -> Prop :=
-| sta0_wf_nil : sta0_wf nil
-| sta0_wf_cons Γ A s l :
-  sta0_wf Γ ->
-  sta0_type Γ A (Sort s l) ->
-  sta0_wf (A :: Γ).
-
-Scheme sta0_type_mut := Induction for sta0_type Sort Prop
-with sta0_wf_mut := Induction for sta0_wf Sort Prop.
-
-Lemma sta0_type_wf Γ m A : sta0_type Γ m A -> sta0_wf Γ.
-Proof with eauto. elim=>{Γ m A}... Qed.
-#[global] Hint Resolve sta0_type_wf.
-
 Reserved Notation "Γ ⊢ m : A" (at level 50, m, A at next level).
 Inductive sta_type : sta_ctx -> term -> term -> Prop :=
-| sta_axiom Γ s l :
+| sta_axiom Γ :
   sta_wf Γ ->
-  Γ ⊢ Sort s l : Sort U l.+1
+  Γ ⊢ Ty : Ty
 | sta_var Γ x A :
   sta_wf Γ ->
   sta_has Γ x A ->
   Γ ⊢ Var x : A
-| sta_pi0 Γ A B s r t l1 l2 :
-  Γ ⊢ A : Sort r l1 ->
-  (A :: Γ) ⊢ B : Sort t l2 ->
-  Γ ⊢ Pi0 A B s : Sort s (maxn l1 l2)
-| sta_pi1 Γ A B s r t l1 l2 :
-  Γ ⊢ A : Sort r l1 ->
-  (A :: Γ) ⊢ B : Sort t l2 ->
-  Γ ⊢ Pi1 A B s : Sort s (maxn l1 l2)
-| sta_lam0 Γ A B m s :
+| sta_forall Γ A B :
+  Γ ⊢ A : Ty ->
+  (A :: Γ) ⊢ B : Ty ->
+  Γ ⊢ Forall A B : Ty
+| sta_arrow Γ A B :
+  Γ ⊢ A : Ty ->
+  (A :: Γ) ⊢ B.[ren (+1)] : Ty ->
+  Γ ⊢ Arrow A B : Ty
+| sta_lam Γ A B m :
+  Γ ⊢ A : Ty ->
   (A :: Γ) ⊢ m : B ->
-  Γ ⊢ Lam0 A m s : Pi0 A B s
-| sta_lam1 Γ A B m s :
-  (A :: Γ) ⊢ m : B ->
-  Γ ⊢ Lam1 A m s : Pi1 A B s
-| sta_app0 Γ A B m n s :
-  Γ ⊢ m : Pi0 A B s ->
+  Γ ⊢ Lam A m : Forall A B
+| sta_fun Γ A B m :
+  Γ ⊢ A : Ty ->
+  (A :: Γ) ⊢ m : B.[ren (+1)] ->
+  Γ ⊢ Fun A m : Arrow A B
+| sta_inst Γ A B m n :
+  Γ ⊢ m : Forall A B ->
   Γ ⊢ n : A ->
-  Γ ⊢ App m n : B.[n/]
-| sta_app1 Γ A B m n s :
-  Γ ⊢ m : Pi1 A B s ->
+  Γ ⊢ Inst m n : B.[n/]
+| sta_call Γ A B m n :
+  Γ ⊢ m : Arrow A B ->
   Γ ⊢ n : A ->
-  Γ ⊢ App m n : B.[n/]
-| sta_sig0 Γ A B s r t l1 l2 :
-  s ⊑ t ->
-  Γ ⊢ A : Sort s l1 ->
-  (A :: Γ) ⊢ B : Sort r l2 ->
-  Γ ⊢ Sig0 A B t : Sort t (maxn l1 l2)
-| sta_sig1 Γ A B s r t l1 l2 :
-  s ⊑ t ->
-  r ⊑ t ->
-  Γ ⊢ A : Sort s l1 ->
-  (A :: Γ) ⊢ B : Sort r l2 ->
-  Γ ⊢ Sig1 A B t : Sort t (maxn l1 l2)
-| sta_pair0 Γ A B m n t l :
-  Γ ⊢ Sig0 A B t : Sort t l ->
-  Γ ⊢ m : A ->
-  Γ ⊢ n : B.[m/] ->
-  Γ ⊢ Pair0 m n t : Sig0 A B t
-| sta_pair1 Γ A B m n t l :
-  Γ ⊢ Sig1 A B t : Sort t l ->
-  Γ ⊢ m : A ->
-  Γ ⊢ n : B.[m/] ->
-  Γ ⊢ Pair1 m n t : Sig1 A B t
-| sta_letin0 Γ A B C m n s t l :
-  (Sig0 A B t :: Γ) ⊢ C : Sort s l ->
-  Γ ⊢ m : Sig0 A B t ->
-  (B :: A :: Γ) ⊢ n : C.[Pair0 (Var 1) (Var 0) t .: ren (+2)] ->
-  Γ ⊢ LetIn C m n : C.[m/]
-| sta_letin1 Γ A B C m n s t l :
-  (Sig1 A B t :: Γ) ⊢ C : Sort s l ->
-  Γ ⊢ m : Sig1 A B t ->
-  (B :: A :: Γ) ⊢ n : C.[Pair1 (Var 1) (Var 0) t .: ren (+2)] ->
-  Γ ⊢ LetIn C m n : C.[m/]
-| sta_with Γ A B s r t l1 l2 :
-  Γ ⊢ A : Sort s l1 ->
-  Γ ⊢ B : Sort r l2 ->
-  Γ ⊢ With A B t : Sort t (maxn l1 l2)
-| sta_apair Γ A B m n t :
-  Γ ⊢ m : A ->
-  Γ ⊢ n : B ->
-  Γ ⊢ APair m n t : With A B t
-| sta_fst Γ A B m t :
-  Γ ⊢ m : With A B t ->
-  Γ ⊢ Fst m : A
-| sta_snd Γ A B m t :
-  Γ ⊢ m : With A B t ->
-  Γ ⊢ Snd m : B
-| sta_id Γ A m n s l :
-  Γ ⊢ A : Sort s l ->
-  Γ ⊢ m : A ->
-  Γ ⊢ n : A ->
-  Γ ⊢ Id A m n : Sort U l
-| sta_refl Γ A m :
-  Γ ⊢ m : A ->
-  Γ ⊢ Refl m : Id A m m
-| sta_rw Γ A B H P m n s l :
-  (Id A.[ren (+1)] m.[ren (+1)] (Var 0) :: A :: Γ) ⊢ B : Sort s l ->
-  Γ ⊢ H : B.[Refl m,m/] ->
-  Γ ⊢ P : Id A m n ->
-  Γ ⊢ Rw B H P : B.[P,n/]
-| sta_conv Γ A B m s l :
+  Γ ⊢ Call m n : B
+| sta_unitT Γ :
+  sta_wf Γ ->
+  Γ ⊢ UnitT : Ty
+| sta_unit Γ :
+  sta_wf Γ ->
+  Γ ⊢ Unit : UnitT
+| sta_natT Γ :
+  sta_wf Γ ->
+  Γ ⊢ NatT : Ty
+| sta_nat Γ n :
+  sta_wf Γ ->
+  Γ ⊢ Nat n : NatT
+| sta_rand Γ m :
+  Γ ⊢ m : UnitT ->
+  Γ ⊢ Rand m : NatT
+| sta_conv Γ A B m :
   A === B ->
   Γ ⊢ m : A ->
-  Γ ⊢ B : Sort s l ->
+  Γ ⊢ B : Ty ->
   Γ ⊢ m : B
 where "Γ ⊢ m : A" := (sta_type Γ m A)
 
 with sta_wf : sta_ctx -> Prop :=
 | sta_wf_nil : sta_wf nil
-| sta_wf_cons Γ A s l :
+| sta_wf_cons Γ A :
   sta_wf Γ ->
-  Γ ⊢ A : Sort s l ->
+  Γ ⊢ A : Ty ->
   sta_wf (A :: Γ).
 
 Scheme sta_type_mut := Induction for sta_type Sort Prop
 with sta_wf_mut := Induction for sta_wf Sort Prop.
 
 Lemma sta_type_wf Γ m A : Γ ⊢ m : A -> sta_wf Γ.
-Proof with eauto.
-  elim=>{Γ m A}...
-  { move=>Γ A _ _ _ _ wf. inv wf... }
-  { move=>Γ A _ _ _ _ wf. inv wf... }
-Qed.
+Proof with eauto. elim=>{Γ m A}... Qed.
 #[global] Hint Resolve sta_type_wf.
 
-Lemma sta_sta0_type Γ m A : Γ ⊢ m : A -> sta0_type Γ m A.
-Proof with eauto using sta0_type, sta0_wf.
-  move:Γ m A. apply:(@sta_type_mut _ (fun Γ wf => sta0_wf Γ))...
-  { move=>Γ A B m s tym ihm.
-    have wf0:=sta0_type_wf ihm. inv wf0.
-    apply: sta0_lam0... }
-  { move=>Γ A B m s tym ihm.
-    have wf0:=sta0_type_wf ihm. inv wf0.
-    apply: sta0_lam1... }
-  Unshelve. eauto.
-  Unshelve. eauto.
-Qed.
-#[global] Hint Resolve sta_sta0_type.
-
-Lemma sta0_sta_type Γ m A : sta0_type Γ m A -> Γ ⊢ m : A.
-Proof with eauto using sta_type, sta_wf.
-  move:Γ m A. apply:(@sta0_type_mut _ (fun Γ wf => sta_wf Γ))...
-  Unshelve. eauto.
-  Unshelve. eauto.
-Qed.
