coq_effect/dyn_prog.v
@@ -1,0 +1,81 @@
+From mathcomp Require Import ssreflect ssrbool eqtype ssrnat seq.
+From Coq Require Import ssrfun Classical Utf8.
+Require Export AutosubstSsr ARS dyn_sr.
+
+Set Implicit Arguments.
+Unset Strict Implicit.
+Unset Printing Implicit Defensive.
+
+Ltac inv_dyn_val :=
+  match goal with
+  | [ H : dyn_val _ |- _ ] => inv H
+  end.
+
+Lemma dyn_forall_canonical m A B C :
+  nil ⊢ m : C -> C === Forall A B -> dyn_val m ->
+  exists A n, m = Lam A n.
+Proof with eauto.
+  move e:(nil)=>Γ ty. elim: ty e A B=>{Γ m C}.
+  all: try solve[intros; exfalso; (solve_conv||inv_dyn_val)].
+  { move=>Γ A B m tyA ihA tym ihm e A0 B0 eq v. subst.
+    exists A. exists m... }
+  { move=>Γ A B m eq1 tym ihm tyB ihB e A0 B0 eq2 vl. subst.
+    apply: ihm...
+    apply: conv_trans... }
+Qed.
+
+Lemma dyn_arrow_canonical m A B C :
+  nil ⊢ m : C -> C === Arrow A B -> dyn_val m ->
+  exists A n, m = Fun A n.
+Proof with eauto.
+  move e:(nil)=>Γ ty. elim: ty e A B=>{Γ m C}.
+  all: try solve[intros; exfalso; (solve_conv||inv_dyn_val)].
+  { move=>Γ A B m tyA ihA tym ihm e1 A0 B0 eq v. subst.
+    exists A. exists m... }
+  { move=>Γ A B m eq1 tym ihm tyB ihB e A0 B0 eq2 vl.
+    apply: ihm...
+    apply: conv_trans... }
+Qed.
+
+Lemma dyn_unit_canonical m C :
+  nil ⊢ m : C -> C === UnitT -> dyn_val m -> m = Unit.
+Proof with eauto.
+  move e:(nil)=>Γ ty. elim: ty e=>{Γ m C}.
+  all: try solve[intros; exfalso; (solve_conv||inv_dyn_val)]...
+  { move=>Γ A B m eq1 tym ihm tyB ihB e eq2 vl. subst.
+    apply: ihm...
+    apply: conv_trans... }
+Qed.
+
+Lemma dyn_prog m A : nil ⊢ m : A -> (exists n, m ~>> n) \/ dyn_val m.
+Proof with eauto using sta_step, dyn_step, dyn_val.
+  move e:(nil)=>Γ ty. elim: ty e=>{Γ m A}.
+  { move=>Γ wf e. right... }
+  { move=>Γ x A wf shs e. subst. inv shs. }
+  { move=>*. right... }
+  { move=>*. right... }
+  { move=>*. right... }
+  { move=>*. right... }
+  { move=>Γ A B m n tym ihm tyn ihn e. subst.
+    have[[m0 st]|v]:=ihm erefl.
+    { left. exists (Inst m0 n)... }
+    { have[A0[n0 e]]:=dyn_forall_canonical tym (convR _ _) v. subst.
+      left. exists (n0.[n/])... } }
+  { move=>Γ A B m n tym ihm tyn ihn e. subst.
+    have[[m0 st]|v]:=ihm erefl.
+    { left. exists (Call m0 n)... }
+    { have[A0[m0 e]]:=dyn_arrow_canonical tym (convR _ _) v. subst.
+      have[[n0 st]|v0]:=ihn erefl.
+      left. exists (Call (Fun A0 m0) n0)...
+      left. exists (m0.[n/])... } }
+  { move=>Γ wf e. right... }
+  { move=>Γ wf e. right... }
+  { move=>Γ wf e. right... }
+  { move=>Γ wf e. right... }
+  { move=>Γ m tym ihm e. subst.
+    have[[n st]|v]:=ihm erefl.
+    left. exists (Rand n)...
+    have e:=dyn_unit_canonical tym (convR _ _) v. subst.
+    left. exists (Nat 0). constructor. }
+  { move=>Γ A B m eq tym ihm tyB ihB e. subst... }
+Qed.
