coq_effect/dyn_sr.v
@@ -1,0 +1,47 @@
+From mathcomp Require Import ssreflect ssrbool eqtype ssrnat seq.
+From Coq Require Import ssrfun Classical Utf8.
+Require Export AutosubstSsr ARS sta_sr dyn_step.
+
+Set Implicit Arguments.
+Unset Strict Implicit.
+Unset Printing Implicit Defensive.
+
+Theorem dyn_sr Γ m n A : Γ ⊢ m : A -> m ~>> n -> Γ ⊢ n : A.
+Proof with eauto using sta_type, sta_wf, sta_step, dyn_step, sta_sr.
+  move=>ty. elim: ty n=>{Γ m A}.
+  { move=>Γ wf n st. inv st. }
+  { move=>Γ x A wf hs n st. inv st. }
+  { move=>Γ A B tyA ihA tyB ihB n st. inv st. }
+  { move=>Γ A B tyA ihA tyB ihB n st. inv st. }
+  { move=>Γ A B m tyA ihA tym ihm n st. inv st. }
+  { move=>Γ A B m tyA ihA tym ihm n st. inv st. }
+  { move=>Γ A B m n tym ihm tyn ihn x st. inv st.
+    { have tym':=ihm _ H2... }
+    { have tyn':=sta_sr tyn H2.
+      have/sta_forall_inv[tyB _]:=sta_valid tym.
+      apply: sta_conv.
+      apply: sta_conv_beta.
+      apply: conv1i...
+      apply: sta_inst...
+      apply: sta_esubst...
+      by autosubst. }
+    { have tyP:=sta_valid tym.
+      have/sta_lam_inv tym0:= tym.
+      apply: sta_esubst... } }
+  { move=>Γ A B m n tym ihm tyn ihn x st. inv st.
+    { have tym':=ihm _ H2... }
+    { have tyn':=ihn _ H2.
+      apply: sta_call... }
+    { have tyP:=sta_valid tym.
+      have/sta_fun_inv tym0:= tym.
+      apply: sta_esubst...
+      by autosubst. } }
+  { move=>Γ wf n st. inv st. }
+  { move=>Γ wf n st. inv st. }
+  { move=>Γ wf n st. inv st. }
+  { move=>Γ n wf n0 st. inv st. }
+  { move=>Γ m tym ihm n st. inv st... }
+  { move=>Γ A B m eq tym ihm tyB ihB n st.
+    apply: sta_conv... }
+Qed.
+
