coq_effect/dyn_step.v
@@ -1,0 +1,56 @@
+From mathcomp Require Import ssreflect ssrbool eqtype ssrnat seq.
+From Coq Require Import ssrfun Classical Utf8.
+Require Export AutosubstSsr ARS etl_ast sta_step.
+
+Set Implicit Arguments.
+Unset Strict Implicit.
+Unset Printing Implicit Defensive.
+
+Inductive dyn_val : term -> Prop :=
+| dyn_val_ty : 
+  dyn_val Ty
+| dyn_val_forall A B : 
+  dyn_val (Forall A B)
+| dyn_val_arrow A B : 
+  dyn_val (Arrow A B)
+| dyn_val_lam A m :
+  dyn_val (Lam A m)
+| dyn_val_fun A m :
+  dyn_val (Fun A m)
+| dyn_val_unitT :
+  dyn_val UnitT
+| dyn_val_unit :
+  dyn_val Unit
+| dyn_val_natT :
+  dyn_val NatT
+| dyn_val_nat n :
+  dyn_val (Nat n).
+
+Reserved Notation "m ~>> n" (at level 50).
+Inductive dyn_step : term -> term -> Prop :=
+| dyn_step_instL m m' n :
+  m ~>> m' ->
+  Inst m n ~>> Inst m' n
+| dyn_step_instR A m n n' :
+  n ~> n' ->
+  Inst (Lam A m) n ~>> Inst (Lam A m) n'
+| dyn_step_betaI A m n :
+  Inst (Lam A m) n ~>> m.[n/]
+| dyn_step_callL m m' n :
+  m ~>> m' ->
+  Call m n ~>> Call m' n
+| dyn_step_callR A m n n' :
+  n ~>> n' ->
+  Call (Fun A m) n ~>> Call (Fun A m) n'
+| dyn_step_betaC A m v :
+  dyn_val v ->
+  Call (Fun A m) v ~>> m.[v/]
+| dyn_step_rand m m' :
+  m ~>> m' ->
+  Rand m ~>> Rand m'
+| dyn_step_randE n :
+  Rand Unit ~>> Nat n
+where "m ~>> n" := (dyn_step m n).
+
+Notation dyn_red := (star dyn_step).
+Notation "m ~>>* n" := (dyn_red m n) (at level 50).
