coq_effect/sta_inv.v
@@ -1,0 +1,37 @@
+From mathcomp Require Import ssreflect ssrbool eqtype ssrnat seq.
+From Coq Require Import ssrfun Classical Utf8.
+Require Export AutosubstSsr ARS sta_subst.
+
+Set Implicit Arguments.
+Unset Strict Implicit.
+Unset Printing Implicit Defensive.
+
+Lemma sta_forall_inv Γ A B C :
+  Γ ⊢ Forall A B : C ->
+  (A :: Γ) ⊢ B : Ty /\ C === Ty.
+Proof with eauto.
+  move e:(Forall A B)=>m ty.
+  elim: ty A B e=>//{Γ C m}.
+  { move=>Γ A B tyA ihA tyB ihB A0 B0 [e1 e2]; subst... }
+  { move=>Γ A B m eq1 tym ihm tyB ihB A0 B0 e; subst.
+    have[tyB0 eq2]:=ihm _ _ erefl.
+    split...
+    apply: conv_trans.
+    apply: conv_sym...
+    exact: eq2. }
+Qed.
+
+Lemma sta_arrow_inv Γ A B C :
+  Γ ⊢ Arrow A B : C ->
+  (A :: Γ) ⊢ B.[ren (+1)] : Ty /\ C === Ty.
+Proof with eauto.
+  move e:(Arrow A B)=>m ty.
+  elim: ty A B e=>//{Γ C m}.
+  { move=>Γ A B tyA ihA tyB ihB A0 B0 [e1 e2]; subst... }
+  { move=>Γ A B m eq1 tym ihm tyB ihB A0 B0 e; subst.
+    have[tyB0 eq2]:=ihm _ _ erefl.
+    split...
+    apply: conv_trans.
+    apply: conv_sym...
+    exact: eq2. }
+Qed.
