coq_effect/sta_valid.v
@@ -1,0 +1,84 @@
+From mathcomp Require Import ssreflect ssrbool eqtype ssrnat seq.
+From Coq Require Import ssrfun Classical Utf8.
+Require Export AutosubstSsr ARS sta_inv.
+
+Set Implicit Arguments.
+Unset Strict Implicit.
+Unset Printing Implicit Defensive.
+
+Theorem sta_valid Γ m A : Γ ⊢ m : A -> Γ ⊢ A : Ty.
+Proof with eauto using sta_type.
+  move=>ty. elim: ty=>{Γ m A}...
+  { move=>Γ x A wf hs.
+    apply: sta_wf_ok... }
+  { move=>Γ A B m n tym ihm tyn ihn.
+    have[tyB _]:=sta_forall_inv ihm.
+    apply: sta_esubst...
+    by autosubst. }
+  { move=>Γ A B m n tym ihm tyn ihn.
+    have[tyB _]:=sta_arrow_inv ihm.
+    apply: sta_esubst...
+    by autosubst.
+    by autosubst. }
+Qed.
+
+Lemma sta_lam_invX Γ A1 A2 B C m :
+  Γ ⊢ Lam A1 m : C ->
+  C === Forall A2 B ->
+  (A2 :: Γ) ⊢ B : Ty ->
+  (A2 :: Γ) ⊢ m : B.
+Proof with eauto.
+  move e:(Lam A1 m)=>n tyL.
+  elim: tyL A1 A2 B m e=>//{Γ C n}.
+  { move=>Γ A B m tyA ihA tym _ A1 A2 B0 m0[e1 e2]/forall_inj[e3 e4]tyB0; subst.
+    have wf:=sta_type_wf tym. inv wf.
+    have wf:=sta_type_wf tyB0. inv wf.
+    apply: sta_ctx_conv.
+    apply: conv_sym...
+    exact: H4.
+    apply: sta_conv...
+    apply: sta_ctx_conv... }
+  { move=>Γ A B m eq1 tym ihm tyB ihB A1 A2 B0 m0 e eq2 tyB0; subst.
+    apply: ihm...
+    apply: conv_trans... }
+Qed.
+
+Lemma sta_fun_invX Γ A1 A2 B C m :
+  Γ ⊢ Fun A1 m : C ->
+  C === Arrow A2 B ->
+  (A2 :: Γ) ⊢ B.[ren (+1)] : Ty ->
+  (A2 :: Γ) ⊢ m : B.[ren (+1)].
+Proof with eauto.
+  move e:(Fun A1 m)=>n tyL.
+  elim: tyL A1 A2 B m e=>//{Γ C n}.
+  { move=>Γ A B m tyA ihA tym _ A1 A2 B0 m0[e1 e2]/arrow_inj[e3 e4]tyB0; subst.
+    have wf:=sta_type_wf tym. inv wf.
+    have wf:=sta_type_wf tyB0. inv wf.
+    apply: sta_ctx_conv.
+    apply: conv_sym...
+    exact: H4.
+    apply: sta_conv.
+    apply: sta_conv_subst.
+    apply: e4.
+    apply: tym.
+    apply: sta_ctx_conv... }
+  { move=>Γ A B m eq1 tym ihm tyB ihB A1 A2 B0 m0 e eq2 tyB0; subst.
+    apply: ihm...
+    apply: conv_trans... }
+Qed.
+
+Lemma sta_lam_inv Γ m A1 A2 B :
+  Γ ⊢ Lam A2 m : Forall A1 B -> (A1 :: Γ) ⊢ m : B.
+Proof with eauto.
+  move=>ty.
+  have/sta_forall_inv[tyB _]:=sta_valid ty.
+  apply: sta_lam_invX...
+Qed.
+
+Lemma sta_fun_inv Γ m A1 A2 B :
+  Γ ⊢ Fun A2 m : Arrow A1 B -> (A1 :: Γ) ⊢ m : B.[ren (+1)].
+Proof with eauto.
+  move=>ty.
+  have/sta_arrow_inv[tyB _]:=sta_valid ty.
+  apply: sta_fun_invX...
+Qed.
