coq_effect/sta_weak.v
@@ -1,0 +1,148 @@
+From mathcomp Require Import ssreflect ssrbool eqtype ssrnat seq.
+From Coq Require Import ssrfun Classical Utf8.
+Require Export AutosubstSsr ARS sta_ctx sta_type sta_conf.
+
+Set Implicit Arguments.
+Unset Strict Implicit.
+Unset Printing Implicit Defensive.
+
+Inductive sta_agree_ren : (var -> var) ->
+  sta_ctx -> sta_ctx -> Prop :=
+| sta_agree_ren_nil ξ :
+  sta_agree_ren ξ nil nil
+| sta_agree_ren_cons Γ Γ' ξ m :
+  Γ ⊢ m : Ty ->
+  sta_agree_ren ξ Γ Γ' ->
+  sta_agree_ren (upren ξ) (m :: Γ) (m.[ren ξ] :: Γ')
+| sta_agree_ren_wk Γ Γ' ξ m :
+  Γ' ⊢ m : Ty ->
+  sta_agree_ren ξ Γ Γ' ->
+  sta_agree_ren (ξ >>> (+1)) (Γ) (m :: Γ').
+
+Lemma sta_agree_ren_refl Γ : sta_wf Γ -> sta_agree_ren id Γ Γ.
+Proof with eauto using sta_agree_ren.
+  move=>wf. elim: wf=>{Γ}...
+  move=>Γ A wf agr tyA.
+  have:(sta_agree_ren (upren id) (A :: Γ) (A.[ren id] :: Γ))...
+  by asimpl.
+Qed.
+
+Lemma sta_agree_ren_has Γ Γ' ξ x A :
+  sta_agree_ren ξ Γ Γ' -> sta_has Γ x A -> sta_has Γ' (ξ x) A.[ren ξ].
+Proof with eauto.
+  move=>agr. elim: agr x A=>{Γ Γ' ξ}.
+  { move=>ξ x A hs. inv hs. }
+  { move=>Γ Γ' ξ m tym agr ih x A hs. inv hs; asimpl.
+    { replace m.[ren (ξ >>> (+1))] with m.[ren ξ].[ren (+1)] by autosubst.
+      constructor. }
+    { replace A0.[ren (ξ >>> (+1))] with A0.[ren ξ].[ren (+1)] by autosubst.
+      constructor... } }
+  { move=>Γ Γ' ξ m tym agr ih x B /ih hs. asimpl.
+    replace B.[ren (ξ >>> (+1))] with B.[ren ξ].[ren (+1)] by autosubst.
+    constructor... }
+Qed.
+
+Lemma sta_agree_weak_wf_nil Γ' ξ : sta_agree_ren ξ nil Γ' -> sta_wf Γ'.
+Proof with eauto using sta_wf.
+  move e:(nil)=>Γ agr. elim: agr e=>//{Γ Γ' ξ}...
+Qed.
+
+Lemma sta_agree_weak_wf_cons Γ Γ' A ξ :
+  sta_agree_ren ξ (A :: Γ) Γ' -> sta_wf Γ -> 
+  (∀ Γ' ξ, sta_agree_ren ξ Γ Γ' → sta_wf Γ') ->
+  (∀ Γ' ξ, sta_agree_ren ξ Γ Γ' → Γ' ⊢ A.[ren ξ] : Ty) ->
+  sta_wf Γ'.
+Proof with eauto using sta_wf.
+  move e:(A :: Γ)=>Γ0 agr. elim: agr Γ A e=>//{Γ0 Γ' ξ}...
+  move=>Γ Γ' ξ m tym agr _ Γ0 A [e1 e2] wf h1 h2; subst.
+  have tym':=h2 _ _ agr.
+  apply: sta_wf_cons...
+Qed.
+
+Lemma sta_rename Γ Γ' m A ξ :
+  Γ ⊢ m : A -> sta_agree_ren ξ Γ Γ' -> Γ' ⊢ m.[ren ξ] : A.[ren ξ].
+Proof with eauto using sta_type, sta_wf, sta_agree_ren.
+  move=>tym. move:Γ m A tym Γ' ξ.
+  apply:(@sta_type_mut _ (fun Γ wf => forall Γ' ξ, sta_agree_ren ξ Γ Γ' -> sta_wf Γ'))...
+  { move=>Γ x A wf h hs Γ' ξ agr. asimpl.
+    apply: sta_var...
+    apply: sta_agree_ren_has... }
+  { move=>Γ A B tyA ihA tyB ihB Γ' ξ agr. asimpl.
+    have wf:=sta_type_wf tyB. inv wf.
+    apply: sta_forall... }
+  { move=>Γ A B tyA ihA tyB ihB Γ' ξ agr. asimpl.
+    have wf:=sta_type_wf tyB. inv wf.
+    have{}ihB:=ihB _ _ (sta_agree_ren_cons H2 agr).
+    asimpl in ihB.
+    apply: sta_arrow...
+    by asimpl. }
+  { move=>Γ A B m tyA ihA tym ihm Γ' ξ agr. asimpl.
+    have wf:=sta_type_wf tym. inv wf.
+    apply: sta_lam... }
+  { move=>Γ A B m tyA ihA tym ihm Γ' ξ agr. asimpl.
+    have wf:=sta_type_wf tym. inv wf.
+    have{}ihm:=ihm _ _ (sta_agree_ren_cons H2 agr).
+    asimpl in ihm.
+    apply: sta_fun...
+    by asimpl. }
+  { move=>Γ A B m n tym ihm tyn ihn Γ' ξ agr. asimpl.
+    replace B.[n.[ren ξ] .: ren ξ] with B.[ren (upren ξ)].[n.[ren ξ]/]
+      by autosubst.
+    have{}ihm:=ihm _ _ agr.
+    have{}ihn:=ihn _ _ agr.
+    apply: sta_inst...
+    asimpl in ihm... }
+  { move=>Γ A B m eq tym ihm tyB ihB Γ' ξ agr.
+    apply: sta_conv.
+    apply: sta_conv_subst.
+    apply: eq.
+    by apply: ihm.
+    have:=ihB _ _ agr.
+    asimpl... }
+  { exact: sta_agree_weak_wf_nil. }
+  { move=>Γ A wf ih tyA ihA Γ' ξ agr.
+    apply: sta_agree_weak_wf_cons... }
+Qed.
+
+Lemma sta_rename_wf Γ Γ' ξ :
+  sta_wf Γ -> sta_agree_ren ξ Γ Γ' -> sta_wf Γ'.
+Proof with eauto using sta_wf.
+  move=>wf. elim: wf Γ' ξ=>{Γ}.
+  { move=>*. apply: sta_agree_weak_wf_nil... }
+  { move=>Γ A wf ih tyA Γ' ξ agr.
+    apply: sta_agree_weak_wf_cons...
+    move=>Γ'0 ξ0 agr0.
+    have:= sta_rename tyA agr0.
+    by autosubst. }
+Qed.
+
+Lemma sta_wf_ok Γ x A :
+  sta_wf Γ -> sta_has Γ x A -> Γ ⊢ A : Ty.
+Proof with eauto using sta_agree_ren, sta_agree_ren_refl.
+  move=>wf. elim: wf x A=>{Γ}.
+  { move=>x A hs. inv hs. }
+  { move=>Γ A wf ih tyA x B hs. inv hs.
+    { replace Ty with Ty.[ren (+1)] by autosubst.
+      apply: sta_rename... }
+    { have tyA0:=ih _ _ H3.
+      replace Ty with Ty.[ren (+1)] by autosubst.
+      apply: sta_rename... } }
+Qed.
+
+Lemma sta_weaken Γ m A B :
+  Γ ⊢ m : A ->
+  Γ ⊢ B : Ty ->
+  (B :: Γ) ⊢ m.[ren (+1)] : A.[ren (+1)].
+Proof with eauto using sta_agree_ren, sta_agree_ren_refl.
+  move=>tym tyB. apply: sta_rename...
+Qed.
+
+Lemma sta_eweaken Γ m m' A A' B :
+  m' = m.[ren (+1)] ->
+  A' = A.[ren (+1)] ->
+  Γ ⊢ m : A ->
+  Γ ⊢ B : Ty ->
+  (B :: Γ) ⊢ m' : A'.
+Proof with eauto using sta_agree_ren, sta_agree_ren_refl.
+  move=>*; subst. apply: sta_weaken...
+Qed.
